NoChangeOwner LTL in

michael_formal/EFSM_LTL.thy
@@ -1,8 +1,21 @@
 theory EFSM_LTL
 imports EFSM "~~/src/HOL/Library/Linear_Temporal_Logic_on_Streams" Filesystem
 begin
-type_synonym full_observation = "(statename option \<times> datastate \<times> event \<times> outputs) stream"
+
+record state =
+  statename :: "statename option"
+  datastate :: datastate
+  event :: event
+  "output" :: outputs
+
+type_synonym full_observation = "state stream"
 type_synonym property = "full_observation \<Rightarrow> bool"
+
+abbreviation label :: "state \<Rightarrow> string" where
+  "label s \<equiv> fst (event s)"
+
+abbreviation inputs :: "state \<Rightarrow> int list" where
+  "inputs s \<equiv> snd (event s)"
 
 fun ltl_step :: "efsm \<Rightarrow> statename option \<Rightarrow> datastate \<Rightarrow> event \<Rightarrow> (statename option \<times> outputs \<times> datastate)" where
 "ltl_step _ None r _ = (None, [], r)" |
@@ -12,13 +25,13 @@ fun ltl_step :: "efsm \<Rightarrow> statename option \<Rightarrow> datastate \<R
   )"
 
 primcorec make_full_observation :: "efsm \<Rightarrow> statename option \<Rightarrow> datastate \<Rightarrow> event stream \<Rightarrow> full_observation" where
-  "make_full_observation e s d i = (let (s', o', d') = ltl_step e s d (shd i) in (s, d, (shd i), o')##(make_full_observation e s' d' (stl i)))"
+  "make_full_observation e s d i = (let (s', o', d') = ltl_step e s d (shd i) in \<lparr>statename = s, datastate = d, event=(shd i), output = o'\<rparr>##(make_full_observation e s' d' (stl i)))"
 
 abbreviation one_or_2 :: "full_observation \<Rightarrow> bool" where
-  "one_or_2 s \<equiv> ((fst (shd s)) = Some 1 \<or> (fst (shd s)) = Some 2)"
+  "one_or_2 s \<equiv> ((statename (shd s)) = Some 1 \<or> (statename (shd s)) = Some 2)"
 
 abbreviation none :: "full_observation \<Rightarrow> bool" where
-  "none s \<equiv> ((fst (shd s)) = None)"
+  "none s \<equiv> ((statename (shd s)) = None)"
 
 lemma "UNTIL one_or_2 none (make_full_observation filesystem (Some 1) <> i)"
 proof (coinduction)
@@ -34,31 +47,32 @@ abbreviation watch_filesystem :: "event stream \<Rightarrow> full_observation" w
   "watch_filesystem i \<equiv> (make_full_observation filesystem (Some 1) <> i)"
 
 fun label_not_logout :: property where
-  "label_not_logout ((s, d, (l, i), p)##t) = (l \<noteq> ''logout'')"
+  "label_not_logout (h##t) = (label h \<noteq> ''logout'')"
 
 fun label_logout :: property where
-  "label_logout ((s, d, (l, i), p)##t) = (l = ''logout'')"
+  "label_logout (h##t) = (label h = ''logout'')"
 
 fun label_create :: property where
-  "label_create ((s, d, (l, i), p)##t) = (l = ''create'')"
+  "label_create (h##t) = (label h = ''create'')"
 
 fun read_0 :: property where
-  "read_0 ((s, d, (l, i), p)##t) = (l=''read'' \<longrightarrow> p=[0])"
+  "read_0 (h##t) = (label h=''read'' \<longrightarrow> output h=[0])"
 
 fun login_attacker :: property where
-  "login_attacker ((s, d, (l, i), p)##t) = (l = ''read'' \<and> i = [1])"
+  "login_attacker (h##t) = (event h = (''login'',  [1]))"
 
 fun login_user :: property where
-  "login_user ((s, d, (l, i), p)##t) = (l = ''read'' \<and> i = [0])"
+  "login_user (h##t) = (event h = (''login'',  [0]))"
 
 fun non_null :: property where
-  "non_null ((s, d, (l, i), p)##t) = (s \<noteq> None)"
+  "non_null (h##t) = (statename h \<noteq> None)"
 
-lemma "alw ((login_attacker aand ev label_logout) impl (read_0 until label_logout)) (make_full_observation filesystem (Some 1) <> i)"
-  sorry (* This is false but is a part of the formula that we actually want *)
+lemma "login_user (watch_filesystem i) \<Longrightarrow> shd i = (''login'', [0])"
+  by (metis login_user.elims(2) make_full_observation.simps(1) state.select_convs(3) stream.sel(1))
 
+lemma login_user_first: "alw non_null (watch_filesystem i) \<Longrightarrow> (login_user (watch_filesystem i) = (shd i = (''login'', [0])))"
+  by (metis login_user.simps make_full_observation.simps(1) state.select_convs(3) stream.collapse)
       (* G(cfstate /= NULL_STATE)         =>  ((label=login AND ip_1_login_1=(user)) AND U(label/=logout, label=create))                             => F(G(((label=login AND ip_1_login_1=(attacker)) AND F(label=logout))  =>   U(label=read=>X(op_1_read_0=0), label=logout))) *)
 lemma "alw non_null (watch_filesystem i) \<Longrightarrow> login_user (watch_filesystem i)         \<and> ((label_not_logout until label_create) (watch_filesystem i)) \<Longrightarrow> ev (alw ((login_attacker                      aand ev label_logout) impl (read_0 until label_logout))) (watch_filesystem i)"
-  sorry
-
+  apply simp
 end
